\section{Theorie}

\begin{equation}
   \ce{^m_z\symup{A} + ^1_0\symup{n} -> ^{m+1}_z\symup{A}^{\ast} -> ^{m+1}_z \symup{A} + \upgamma } \nonumber
\end{equation}

\begin{equation}
   \ce{^{m+1}_z \symup{A} -> ^{m+1}_{z+1} \symup{C} + \upbeta^- + \symup{E_{kin}} + \bar{\symup{\nu}}_{\symup{e}}} \nonumber
\end{equation}

\begin{equation}
   \Delta E = \Delta m c^2 \nonumber
\end{equation}

\begin{equation}
   \sigma = \frac{u}{nKd} \nonumber
\end{equation}

\begin{equation}
   \lambda = \frac{h}{m_{\symup{n}}v} \nonumber
\end{equation}

\begin{equation}
   \sigma(E) = \sigma_0 \sqrt{ \frac{E_{\symup{r_i}}}{E} } \frac{\tilde{c}}{\left( E - E_{\symup{r_i}} \right)^2 + \tilde{c}} \nonumber
\end{equation}

\begin{equation}
   \sigma \sim \frac{1}{\sqrt{E}} \sim \frac{1}{v} \nonumber
\end{equation}

\begin{equation}
   \ce{ ^9_4 \symup{Be} + ^4_2$\alpha$ -> ^{12}_6\symup{C} + ^1_0\symup{n}} \nonumber
\end{equation}

\begin{equation}
   E_{symup{Ã¼}}  = E_0 \frac{4Mn}{\left( M + m \right)^2} \nonumber
\end{equation}

\begin{equation}
   \ce{^{51} \symup{V}, ^{55}\text{Mn}, ^{79}\text{Br}, ^{115}\text{In}, ^{127}\text{J}, ^{164}\text{Dy}, ^{107}{Ag}, ^{109}\text{Ag}, ^{103}\text{Rh}} \nonumber
\end{equation}

\begin{equation}
   \ce{^{107}_{47}\text{Ag} + \symup{n} -> ^{108}_{47}\text{Ag} -> ^{108}_{48}\text{48} + $\upbeta$^- + \bar{\symup{\nu}}_{\symup{e}}} \nonumber
\end{equation}

\begin{equation}
   \ce{^{109}_{47}\text{Ag} + \symup{n} -> ^{110}_{47}\text{Ag} -> ^{110}_{48}\text{48} + $\upbeta$^- + \bar{\symup{\nu}}_{\symup{e}}} \nonumber
\end{equation}

\begin{equation}
   \begin{split}
      \ce{^{103}_{45}\text{Rh} + \symup{n}} \mathbin{\scalebox{2.5} \textbraceleft } \quad \nonumber
   \end{split}
   \begin{split}
      &\overset{10\%}{\longrightarrow} \ce{^{104\symup{i}}_{45}\text{Rh} -> ^{104}_{45}\text{Rh} + $\upgamma$ -> ^{104}_{46}\text{Pd} + $\upbeta$^- + \bar{\symup{\nu}}_{\symup{e}} } \nonumber\\
      &\overset{90\%}{\longrightarrow} \ce{^{104}_{45}\text{Rh} -> ^{104}_{46}\text{Pd} + $\upbeta$^- +\bar{\symup{\nu}}_{\symup{e}} } \nonumber\\
   \end{split}
\end{equation}

\begin{equation}
   N(t) = N_0 \symup{e}^{- \lambda t} \nonumber
\end{equation}

\begin{equation}
   \frac{N_0}{2} = N_0 \symup{e}^{- \lambda T}  \nonumber
\end{equation}

\begin{equation}
   T = \text{ln}\left(\frac{2}{\lambda}\right) \nonumber
\end{equation}

\begin{equation}
   N_{\Delta t}(t) = N(t) - N(t + \Delta t) \nonumber
\end{equation}

\begin{equation}
   N_{\Delta t}(t) = N_0 \symup{e}^{ - \lambda t} - N_0 \symup{e}^{- \lambda \left( t + \Delta t \right) } = N_0 \left( 1 - \symup{e}^{-\lambda \Delta t} \right) \symup{e}^{-\lambda t} \nonumber
\end{equation}

\begin{equation}
   \text{ln} \left( N_{\Delta t}(t)\right) = \text{ln} \left( N_0 \left( 1- \symup{e}^{-\lambda \Delta t}\right) -\lambda t \right) \nonumber
\end{equation}

\begin{equation}
   \text{ln}\left(N_0\left(1- \symup{e}^{-\lambda\Delta t}\right)  \right) \nonumber
\end{equation}

\begin{equation}
   N_{\Delta t_{l}} \coloneqq N_{0_l}\left( 1- \symup{e}^{-lambda_{l} \Delta t}\right) \symup{e}^{\lambda_l t} \nonumber
\end{equation}

\begin{equation}
   N_{\Delta t}(t_{\symup{i}}) - N_{\Delta t_l}(t_{\symup{i}}) \leq 0 \nonumber
\end{equation}

\begin{equation}
   N_{\Delta t} (t_{\symup{i}}) = N_{\Delta t , \text{gem}}(t_{\symup{i}}) - N_{\Delta t, \symup{u}} \nonumber
\end{equation}